theories/zoo/common/string.v
@@ -1,0 +1,20 @@
+From stdpp Require Export
+  strings.
+
+From zoo Require Import
+  prelude.
+From zoo Require Import
+  options.
+
+#[local] Fixpoint split_on_go chr str acc :=
+  match str with
+  | "" =>
+      (String.rev acc, None)
+  | String chr' str =>
+      if Ascii.eqb chr chr' then
+        (String.rev acc, Some str)
+      else
+      split_on_go chr str (String chr' acc)
+  end.
+Definition split_on chr str :=
+  split_on_go chr str "".
